src/QUIC.fst
@@ -1,0 +1,97 @@
+module QUIC
+
+module QSpec = QUIC.Spec
+module QImpl = QUIC.Impl
+module QImplBase = QUIC.Impl.Base
+module QModel = Model.QUIC
+
+module I = Model.Indexing
+module G = FStar.Ghost
+module B = LowStar.Buffer
+module S = FStar.Seq
+module HS = FStar.HyperStack
+module ST = FStar.HyperStack.ST
+
+module U64 = FStar.UInt64
+module U32 = FStar.UInt32
+module U8 = FStar.UInt8
+
+open FStar.HyperStack
+open FStar.HyperStack.ST
+
+open EverCrypt.Helpers
+open EverCrypt.Error
+
+let index =
+  if I.model then QModel.id else QImpl.index
+
+let mid (i:index{I.model}) = i <: QModel.id
+let iid (i:index{not I.model}) = i <: QImpl.index
+
+let alg (i:index) =
+  if I.model then I.ae_id_ginfo (fst (mid i))
+  else (iid i).QImpl.aead_alg
+
+let halg (i:index) =
+  if I.model then I.ae_id_ghash (fst (mid i))
+  else (iid i).QImpl.hash_alg
+
+let itraffic_secret (i:QModel.id) =
+  Spec.Hash.Definitions.bytes_hash (I.ae_id_ghash (fst i))
+
+module MH = Model.Helpers
+
+let derived (#i:QModel.id) (#w:QModel.stream_writer i) (r:QModel.stream_reader w) (ts:itraffic_secret i) =
+  if I.model && QModel.unsafe i then
+    let ha = I.ae_id_hash (fst i) in
+    let ea = I.ae_id_info (fst i) in
+    let (k1, k2) = QModel.reader_leak r in
+    QModel.writer_static_iv w ==
+      QSpec.derive_secret ha ts QSpec.label_iv 12 /\
+    k1 == QSpec.derive_secret ha ts
+        QSpec.label_key (QSpec.ae_keysize ea) /\
+    k2 == QUIC.Spec.derive_secret ha ts
+        QUIC.Spec.label_key (QSpec.cipher_keysize ea)
+  else True
+
+noeq type mstate_t i =
+| Ideal:
+  writer: QModel.stream_writer i ->
+  reader: QModel.stream_reader writer ->
+  ts: itraffic_secret i{derived reader ts} -> // FIXME erased
+  mstate_t i
+  
+let istate_t i = QImpl.state i
+
+let state i =
+  if I.model then mstate_t (mid i)
+  else istate_t (iid i)
+
+let mstate (#i:index{I.model}) (s:state i) = s <: mstate_t (mid i)
+let istate (#i:index{not I.model}) (s:state i) = s <: istate_t (iid i)
+
+let footprint #i h s =
+  if I.model then
+    QModel.rfootprint (mstate s).reader
+  else QImpl.footprint h (istate s)
+
+let invariant #i h s =
+  if I.model then
+    QModel.invariant (mstate s).writer h <: Type0
+  else QImpl.invariant h (istate s)
+
+let g_traffic_secret #i s h =
+  if I.model then (mstate s).ts
+  else
+    QImpl.g_traffic_secret (B.deref h (istate s))
+
+let g_initial_packet_number #i s h =
+  if I.model then admit ()
+  else
+    QImpl.g_initial_packet_number (B.deref h (istate s)) h
+
+let g_last_packet_number #i s h =
+  if I.model then
+    QModel.expected_pnT (mstate s).reader h
+  else
+    QImpl.g_last_packet_number (B.deref h (istate s)) h
